tests/monadic/object_model/object_model.h
@@ -10,59 +10,6 @@
 #include <string>
 #include <utility>
 #include <variant>
-#include <vector>
-
-struct Nat {
-  // TYPES
-  struct O {};
-
-  struct S {
-    std::shared_ptr<Nat> a0;
-  };
-
-  using variant_t = std::variant<O, S>;
-
-private:
-  // DATA
-  variant_t v_;
-
-public:
-  // CREATORS
-  Nat() {}
-
-  explicit Nat(O _v) : v_(_v) {}
-
-  explicit Nat(S _v) : v_(std::move(_v)) {}
-
-  static Nat o() { return Nat(O{}); }
-
-  static Nat s(Nat a0) { return Nat(S{std::make_shared<Nat>(std::move(a0))}); }
-
-  // MANIPULATORS
-  ~Nat() {
-    std::vector<std::shared_ptr<Nat>> _stack = {};
-    auto _drain = [&](variant_t &_v) {
-      if (auto *_alt = std::get_if<S>(&_v)) {
-        if (_alt->a0) {
-          _stack.push_back(std::move(_alt->a0));
-        }
-      }
-    };
-    _drain(v_mut());
-    while (!_stack.empty()) {
-      auto _cur = std::move(_stack.back());
-      _stack.pop_back();
-      if (_cur.use_count() == 1) {
-        _drain(_cur->v_mut());
-      }
-    }
-  }
-
-  inline variant_t &v_mut() { return v_; }
-
-  // ACCESSORS
-  const variant_t &v() const { return v_; }
-};
 
 template <typename Err> struct ExceptE {
   // DATA
@@ -94,15 +41,15 @@ concept STRefClass = requires {
 
 struct STRefNat {
   // DATA
-  Nat s;
+  uint64_t s;
 
   // ACCESSORS
   STRefNat clone() const { return {s}; }
 
   // CREATORS
-  static STRefNat mkstref(Nat s) { return {std::move(s)}; }
+  static STRefNat mkstref(uint64_t s) { return {s}; }
 
-  Nat STRefToIxNat() const {
+  uint64_t STRefToIxNat() const {
     const auto &[s] = *this;
     return s;
   }
@@ -116,7 +63,7 @@ template <typename S> struct Point {
 
 template <typename S> struct Account {
   std::function<int64_t(std::monostate)> getBalance;
-  std::function<int64_t(int64_t)> deposit;
+  std::function<int64_t(uint64_t)> deposit;
   std::function<std::optional<int64_t>(int64_t)> withdraw;
 };
 
