tests/monadic/object_model/ObjectModelExtractionTests.v
@@ -120,17 +120,17 @@ Section PointDef.
   
   Record Account := mkAccount {
       getBalance : unit -> itree E0 Z;
-      deposit : Z -> itree E0 Z;
+      deposit : nat -> itree E0 Z;
       withdraw : Z -> itree E0 (option Z);
     }.
 
   Definition getBalance_imp (idx : T) (ref : STRef S Z) : unit -> itree E0 Z :=
     fun _ => readSTRef (idx := idx) ref.
 
-  Definition deposit_imp (idx : T) (ref : STRef S Z) : Z -> itree E0 Z :=
-    fun amt : Z =>
+  Definition deposit_imp (idx : T) (ref : STRef S Z) : nat -> itree E0 Z :=
+    fun amt : nat =>
       bal <- readSTRef (idx := idx) ref;;
-      let new_bal := (bal + amt)%Z in
+      let new_bal := (bal + (Z.of_nat amt))%Z in
       writeSTRef (idx := idx) ref new_bal;;
       Ret new_bal.
 
@@ -151,7 +151,7 @@ Section PointDef.
       {| getBalance _ := !bal_ref;
          deposit amt := 
             bal <- !bal_ref;;
-            let new_bal := (bal + amt)%Z in
+            let new_bal := (bal + (Z.of_nat amt))%Z in
              bal_ref :== new_bal;;
              Ret new_bal;
         withdraw amt := 
@@ -186,7 +186,7 @@ Section PointDef.
     result <- withdraw acc1 a;;
     match result with
     | Some 0%Z => (* withdrawal succeeds, transfer money*)
-        b <- deposit acc2 a;;
+        b <- deposit acc2 (Z.to_nat a);;
         c <- getBalance acc1 tt;;
         Ret (a,true,b,c)
     | _ => (* withdrawal failed, do nothing, return balance of a,b *)
@@ -198,9 +198,7 @@ Section PointDef.
   #[export] Instance hmap_nat_v : HMap (@idx_key T T) (idx_key_type V) mem :=
     HMap_halist (idx_key T) (idx_key_type V).
 
-
   (* TODO: make this a structure instead of `and` *)
-
 
   Definition backed_by (acc : Account) (idx : T) (ref : STRef S Z) : Prop :=
     getBalance acc = getBalance_imp idx ref /\
@@ -330,13 +328,12 @@ Section PointDef.
 
 
   Lemma deposit_preserves_wf :
-    forall (acc : Account) (idx : T) (ref : STRef S Z) (amt new_bal : Z) (m0 m1 : @mem T V) (out_val : Z),
-      (amt >= 0)%Z ->
+    forall (acc : Account) (idx : T) (ref : STRef S Z) (amt : nat) (new_bal : Z) (m0 m1 : @mem T V) (out_val : Z),
       account_wf acc idx ref m0 ->
       interp_st ltu _ (deposit acc amt) m0 ≈ Ret (m1 , out_val) ->
       account_wf acc idx ref m1.
     Proof using Type.
-      intros acc idx ref amt b m0 m1 o Hamt Hwdrw Hintrp.
+      intros acc idx ref amt b m0 m1 o Hwdrw Hintrp.
       unfold account_wf in *. destruct Hwdrw as [Hback Hlookup].
       split; try assumption.
       unfold backed_by in Hback. destruct Hback as [Hgetb [Hwdrw Hdepos]].
@@ -351,7 +348,7 @@ Section PointDef.
       repeat (repeat setoid_rewrite Monad.bind_bind in Hintrp;
           repeat setoid_rewrite bind_Ret_l in Hintrp;
           repeat setoid_rewrite bind_Ret_r in Hintrp).
-      exists (v + amt)%Z. unfold_instances.
+      exists (v + Z.of_nat amt)%Z. unfold_instances.
       change (@Monad.bind (itree ?E) _) with (@ITree.bind E) in Hintrp.
       rewrite interp_st_bind_eutt in Hintrp.
       unfold writeSTRef in Hintrp.
@@ -431,7 +428,7 @@ Proof. lazy. reflexivity. Qed.
 
 
 
-From Crane Require Import Mapping.ZInt.
+From Crane Require Import Mapping.ZInt Mapping.NatIntStd.
 
 Definition testtoST1_ext :=
   Eval unfold testtoST1, class_pointST in (testtoST1 unit).
